Finish preservation for referencing

2016/Referencing.thy
@@ -17,25 +17,31 @@ datatype lterm=
 
 fun shift_L :: "int \<Rightarrow> nat \<Rightarrow> lterm \<Rightarrow> lterm" where
  "shift_L d c (ref t) = ref (shift_L d c t)"|
- "shift_L d c (t1::=t2) = t1::=(shift_L d c t2)"|
+ "shift_L d c (t1::=t2) = (shift_L d c t1)::=(shift_L d c t2)"|
  "shift_L d c (LVar k)    = LVar (if k < c then k else nat (int k + d))" |
  "shift_L d c (LApp t t1) = LApp (shift_L d c t) (shift_L d c t1)" |
  "shift_L d c (LAbs T t)  = LAbs T (shift_L d (Suc c) t)" |
- "shift_L d c t = t" 
+ "shift_L d c (!t) =!(shift_L d c t)" |
+ "shift_L d c unit = unit" | 
+ "shift_L d c (L v) = L v"
 
 fun subst_L :: "nat \<Rightarrow> lterm \<Rightarrow> lterm \<Rightarrow> lterm" where
   "subst_L j s (ref t) = ref (subst_L j s t)"|
-  "subst_L j s (t1::=t2) = t1::=(subst_L j s t2)"|
+  "subst_L j s (t1::=t2) = (subst_L j s t1)::=(subst_L j s t2)"|
   "subst_L j s (LApp t1 t2) = LApp (subst_L j s t1) (subst_L j s t2)" |
   "subst_L j s (LVar k) = (if k = j then s else LVar k)" |
   "subst_L j s (LAbs T t) = LAbs T (subst_L (Suc j) (shift_L 1 0 s) t)"|
-  "subst_L j s t = t"
+  "subst_L j s unit = unit" |
+  "subst_L j s (L n) = L n" |
+  "subst_L j s (!t) = !(subst_L j s t)"
 
 fun FV ::"lterm \<Rightarrow> nat set" where
   "FV (LVar k) = {k}"|
   "FV (LApp t1 t2) = FV t1 \<union> FV t2"|
   "FV (LAbs T t) =  image (\<lambda>x. x - 1) (FV t - {0})" |
-  "FV (t1::=t2) = FV t2"|
+  "FV (t1::=t2) = FV t1 \<union> FV t2"|
+  "FV (ref t) = FV t"|
+  "FV (!t) = FV t"|
   "FV _ = {}"
 
 inductive is_value_L:: "lterm \<Rightarrow> bool" where
@@ -58,15 +64,15 @@ inductive eval1_L :: "lterm \<Rightarrow> lstore \<Rightarrow> lterm \<Rightarro
     "is_value_L v2 \<Longrightarrow> eval1_L (LApp (LAbs T' t12) v2) \<mu>
       (shift_L (-1) 0 (subst_L 0 (shift_L 1 0 v2) t12)) \<mu>" | 
   eval1_LRefV:
-    "is_value_L v \<Longrightarrow> eval1_L (ref v) \<mu> (Loc (length \<mu>)) (\<mu>|\<leftarrow>|v)" |
+    "is_value_L v \<Longrightarrow> eval1_L (ref v) \<mu> (L (length \<mu>)) (\<mu>|\<leftarrow>|v)" |
   eval1_LRef:
     "eval1_L t1 \<mu> t1' \<mu>' \<Longrightarrow> eval1_L (ref t1) \<mu> (ref t1') \<mu>'" |
   eval1_LDerefLoc:
-    "n<length \<mu> \<Longrightarrow> is_value_L (\<mu>!n) \<Longrightarrow> eval1_L (!(Loc n)) \<mu> (\<mu>!n) \<mu>" |
+    "n<length \<mu> \<Longrightarrow>  eval1_L (!(L n)) \<mu> (\<mu>!n) \<mu>" |
   eval1_LDeref:
     "eval1_L t1 \<mu> t1' \<mu>' \<Longrightarrow> eval1_L (!t1) \<mu> (!t1') \<mu>'" |
   eval1_LAssignLoc:
-    "is_value_L v \<Longrightarrow> eval1_L (Loc n::=v) \<mu> unit (\<mu>[n:=v])"|
+    "is_value_L v \<Longrightarrow> eval1_L (L n::=v) \<mu> unit (\<mu>[n:=v])"|
   eval1_LAssign1:
     "eval1_L t1 \<mu> t1' \<mu>' \<Longrightarrow> eval1_L (t1::=t2) \<mu> (t1'::=t2) \<mu>'" |
   eval1_LAssign2:
@@ -124,25 +130,124 @@ by (auto elim: has_type_L.cases is_value_L.cases)
 abbreviation well_typed_store::"lcontext \<Rightarrow> loc_ctx \<Rightarrow> lstore \<Rightarrow> bool" ("(_)|;|(_) \<Turnstile> (_)" [150,150,190] 200) where
 "\<Gamma>|;|\<Sigma> \<Turnstile> \<mu> \<equiv> (length \<Sigma> = length \<mu>) \<and> (\<forall>i<length \<Sigma>. \<Gamma>|;|\<Sigma> \<turnstile> (\<mu>!i) |:| (\<Sigma>!i))"
 
+lemma[simp]: "nat (int x + 1) = Suc x" by simp
+lemma[simp]: "nat (1 + int x) = Suc x" by simp
+lemma[simp]: "nat (int x - 1) = x - 1" by simp
+
+lemma gr_Suc_conv: "Suc x \<le> n \<longleftrightarrow> (\<exists>m. n = Suc m \<and> x \<le> m)"
+  by (cases n) auto
+
+lemma FV_shift:
+  "FV (shift_L (int d) c t) = image (\<lambda>x. if x \<ge> c then x + d else x) (FV t)"
+proof (induction t arbitrary: c rule: lterm.induct)
+  case (LAbs T t)
+  thus ?case  by (auto simp: gr_Suc_conv image_iff) force+
+qed auto
+
+lemma FV_subst:
+  "FV (subst_L n t u) = (if n \<in> FV u then (FV u - {n}) \<union> FV t else FV u)"
+proof (induction u arbitrary: n t rule: lterm.induct)
+  case (LAbs T u)
+  thus ?case 
+    by (auto simp: gr0_conv_Suc image_iff FV_shift[of 1, unfolded int_1],
+        (metis DiffI One_nat_def UnCI diff_Suc_1 empty_iff imageI insert_iff nat.distinct(1))+)
+qed (auto simp: gr0_conv_Suc image_iff FV_shift[of 1, unfolded int_1])
+
+
+lemma weakening:
+  "\<Gamma> |;|\<Sigma> \<turnstile> t |:| T \<Longrightarrow> n \<le> length \<Gamma> \<Longrightarrow> insert_nth n S \<Gamma> |;|\<Sigma> \<turnstile> shift_L 1 n t |:| T"
+proof (induction \<Gamma> \<Sigma> t T arbitrary: n rule: has_type_L.induct)
+  case (has_type_LAbs \<Gamma> T1 t2 T2)
+    from has_type_LAbs.prems has_type_LAbs.hyps
+      has_type_LAbs.IH[where n="Suc n"] 
+    show ?case
+      by (auto intro: has_type_L.intros)
+qed (auto simp: nth_append min_def intro: has_type_L.intros)
+
 lemma substitution:
   "\<Gamma> |;|\<Sigma> \<turnstile> t |:| T \<Longrightarrow>  \<Gamma>|;|\<Sigma> \<turnstile> LVar n |:| S \<Longrightarrow> \<Gamma>|;|\<Sigma> \<turnstile> s |:| S \<Longrightarrow> \<Gamma>|;|\<Sigma> \<turnstile> subst_L n s t |:| T"  
-sorry
+proof (induction \<Gamma> \<Sigma>  t T arbitrary: s n rule: has_type_L.induct)
+  case (has_type_LAbs \<Gamma> T1 \<Sigma> t T2)
+  thus ?case
+    using weakening[where n=0, unfolded insert_nth_def nat.rec]          
+    by (force intro!: has_type_L.intros simp: has_type_L.simps[of _ _ "LVar _" _, simplified])
+qed (auto intro!: has_type_L.intros simp: has_type_L.simps[of _ _ "LVar _" _, simplified])
 
 lemma storing_updt:
   "\<Gamma> |;|\<Sigma> \<Turnstile> \<mu> \<Longrightarrow> i<length \<Sigma> \<Longrightarrow> \<Sigma>!i = T \<Longrightarrow> \<Gamma> |;|\<Sigma> \<turnstile> v |:| T \<Longrightarrow> \<Gamma> |;|\<Sigma> \<Turnstile> (\<mu>[i:=v])"
-sorry
-
+by (simp, metis  nth_list_update_eq nth_list_update_neq)
+       
 lemma store_weakening:
   "\<Gamma> |;|\<Sigma> \<turnstile> t |:| T \<Longrightarrow> \<Gamma>|;|(\<Sigma>@\<Sigma>1) \<turnstile> t |:| T" 
-sorry
+by (induction \<Gamma> \<Sigma>  t T arbitrary: \<Sigma>1 rule: has_type_L.induct)
+   (auto intro!: has_type_L.intros 
+         simp: has_type_L.simps[of _ _ "LVar _" _, simplified] nth_append)
 
 lemma progress:
-  "\<emptyset>|;|\<Sigma> \<turnstile> t |:| T \<Longrightarrow> is_value_L t \<or> (\<forall>\<mu>. \<emptyset>|;|\<Sigma> \<Turnstile> \<mu> \<longrightarrow> (\<exists>t' \<mu>'. eval1_L t \<mu> t' \<mu>'))"
-sorry
+  "\<Gamma>|;|\<Sigma> \<turnstile> t |:| T \<Longrightarrow> \<Gamma>=\<emptyset> \<Longrightarrow> is_value_L t \<or> (\<forall>\<mu>. \<Gamma>|;|\<Sigma> \<Turnstile> \<mu> \<longrightarrow> (\<exists>t' \<mu>'. eval1_L t \<mu> t' \<mu>'))"
+proof (induction t T rule: has_type_L.induct)
+  case (has_type_LApp \<Gamma> \<Sigma> t1 T11 T12 t2)
+    note hyps=this
+    show ?case
+      using hyps(3-4)[OF hyps(5)]           
+      by (metis eval1_L.intros(1-3) canonical_forms(2)[OF _ hyps(1)])+
+next
+  case (has_type_Ref \<Gamma> \<Sigma> t T1)
+    note hyps=this
+    show ?case
+      using hyps(2)[OF hyps(3)]
+            eval1_L.intros(4,5)
+      by meson
+next
+  case (has_type_Deref \<Gamma> \<Sigma> t T1)
+    note hyps=this
+    show ?case
+      using hyps(2)[OF hyps(3)] canonical_forms(3)[OF _ hyps(1)]
+            eval1_L.intros(6,7)
+      by metis
+next
+  case (has_type_Assign \<Gamma> \<Sigma> t1 T1 t2)
+    note hyps=this
+    show ?case
+      using hyps(3,4)[OF hyps(5)]
+            canonical_forms(3)[OF _ hyps(1)] eval1_L.intros(8-10)
+      by metis
+qed (simp_all add: is_value_L.intros)
+
+lemma shift_down:
+  "insert_nth n U \<Gamma>|;|\<Sigma> \<turnstile> t |:| T \<Longrightarrow> n \<le> length \<Gamma> \<Longrightarrow>
+   (\<And>x. x \<in> FV t \<Longrightarrow> x \<noteq> n) \<Longrightarrow> \<Gamma>|;|\<Sigma> \<turnstile> shift_L (- 1) n t |:| T"
+proof (induction "insert_nth n U \<Gamma>" \<Sigma> t T arbitrary: \<Gamma> n rule: has_type_L.induct)
+  case (has_type_LAbs V t T)
+    from this(1,3,4) show ?case
+      by (fastforce intro: has_type_L.intros has_type_LAbs.hyps(2)[where n="Suc n"])+
+qed (fastforce intro: has_type_L.intros simp: nth_append min_def)+
+
 
 lemma preservation:
   "\<Gamma> |;|\<Sigma> \<turnstile> t |:| T \<Longrightarrow> \<Gamma> |;|\<Sigma> \<Turnstile> \<mu> \<Longrightarrow> eval1_L t \<mu> t' \<mu>' \<Longrightarrow> 
     \<exists>\<Sigma>1. \<Gamma> |;| (\<Sigma>@\<Sigma>1) \<Turnstile> \<mu>' \<and> \<Gamma> |;|(\<Sigma>@\<Sigma>1) \<turnstile> t' |:| T"
-sorry
+proof (induction \<Gamma> \<Sigma> t T arbitrary: \<mu>' t' rule: has_type_L.induct)
+  case (has_type_LApp \<Gamma> \<Sigma> t1 T11 T12 t2)
+    note hyps = this and has_T_Abs= has_type_L.simps[of _ _ "LAbs _ _", simplified]
+         
+    show ?case
+      using hyps(3,4)[OF hyps(5)]
+            hyps(6)[unfolded eval1_L.simps[of "LApp t1 t2" \<mu>, simplified]]
+      apply auto
+      using has_type_L.intros(4) eval1_L.intros(1,2)
+            hyps(1,2) store_weakening[of \<Gamma> \<Sigma>]
+      apply (meson,meson)
+      using substitution 
+            weakening[where n=0, unfolded insert_nth_def nat.rec]
+            
+      (* by (auto
+      intro!: has_type_L.intros substitution shift_down
+      dest: weakening[where n=0, unfolded insert_nth_def nat.rec]
+      elim!: eval1_LAppE
+      split: lterm.splits if_splits
+      simp: FV_subst FV_shift[of 1, unfolded int_1] has_T_Abs) 
+        (metis neq0_conv)*)
+qed (auto elim: eval1_L.cases)
 
 end
